proof_checking/pxl_completeness_proofs_v4/pxl_phase4_completeness/coq/TEMP_axiom_test.v
@@ -1,0 +1,2 @@
+Definition form := nat -> Type.
+Axiom test_ax : forall (Δ:form) (ψ:nat), True -> True.
